src/util/List.v
@@ -1326,33 +1326,6 @@ Section Existsn.
 End Existsn.
 Hint Constructors Existsn : core.
 
-Inductive filter_Prop {A} (P : A -> Prop) : list A -> list A -> Prop :=
-| filter_Prop_nil : filter_Prop P [] []
-| filter_Prop_keep a l r : P a -> filter_Prop P l r -> filter_Prop P (a :: l) (a :: r)
-| filter_Prop_drop a l r : ~ P a -> filter_Prop P l r -> filter_Prop P (a :: l) r.
-
-Inductive flat_map_Prop {A B} (R : A -> list B -> Prop) : list A -> list B -> Prop :=
-| flat_map_Prop_nil : flat_map_Prop R [] []
-| flat_map_Prop_cons a l bs r :
-  R a bs -> flat_map_Prop R l r -> flat_map_Prop R (a :: l) (bs ++ r).
-
-Lemma flat_map_Prop_perm {A B} (R : A -> list B -> Prop) l1 l2 r1 :
-  Permutation l1 l2 ->
-  flat_map_Prop R l1 r1 ->
-  exists r2, flat_map_Prop R l2 r2 /\ Permutation r1 r2.
-Proof.
-  intros HP. revert r1. induction HP; intros r1 Hf.
-  - invert Hf. exists []. split; [ constructor | reflexivity ].
-  - invert Hf.
-    match goal with H : flat_map_Prop R _ _ |- _ => destruct (IHHP _ H) as (r2 & Hf2 & Hp2) end.
-    eexists. split; [ constructor; [ eassumption | exact Hf2 ] | apply Permutation_app_head; exact Hp2 ].
-  - invert Hf. match goal with H : flat_map_Prop R (_ :: _) _ |- _ => invert H end.
-    eexists. split; [ constructor; [ eassumption | constructor; [ eassumption | eassumption ] ] | ].
-    rewrite !app_assoc. apply Permutation_app_tail. apply Permutation_app_comm.
-  - destruct (IHHP1 _ Hf) as (r2 & Hf2 & Hp2). destruct (IHHP2 _ Hf2) as (r3 & Hf3 & Hp3).
-    exists r3. split; [ assumption | eapply perm_trans; eassumption ].
-Qed.
-
 Section misc.
   Context {A B C D : Type}.
   Implicit Type xs : list A.
